Refactor strict positivity lemma

ReducibilityDefinition.v
@@ -38,7 +38,7 @@ Proof.
   unfold reduces_to; repeat step || eexists; eauto.
 Qed.
 
-Equations (noind) reducible_values (theta: interpretation) (v: tree) (T: tree): Prop
+Equations reducible_values (theta: interpretation) (v: tree) (T: tree): Prop
     by wf (size T, index T) (lexprod _ _ lt lt_index) :=
   reducible_values theta v (fvar X type_var) :=
     match lookup Nat.eq_dec theta X with
